functional-programming-lean/src/type-classes/indexing.md
@@ -1,8 +1,119 @@
-# Indexing
+# Arrays and Indexing
 
 The [Interlude](../props-proofs-indexing.md) describes how to use indexing notation in order to look up entries in a list by their position.
 This syntax is also governed by a type class, and it can be used for a variety of different types.
 
-For instance, Lean arrays are much more efficient that linked lists for most purposes.
+## Arrays
+For instance, Lean arrays are much more efficient than linked lists for most purposes.
+In Lean, the type `Array α` is a dynamically-sized array holding values of type `α`, much like a Java `ArrayList`, a C++ `std::vector`, or a Rust `std::vec`.
+Unlike `List`, arrays occupy a contiguous region of memory, which is much better for processor caches.
+Also, looking up a value in an array takes constant time, while lookup in a linked list takes time proportional to the index being accessed.
 
+In pure functional languages like Lean, it is not possible to mutate a given position in a data structure.
+Instead, a copy is made that has the desired modifications.
+When using an array, the Lean compiler and runtime contain an optimizations that can allow modifications to be implemented as mutations behind the scenes when there is only a single unique reference to an array, while a list would require copies of all prior nodes to be made.
+
+Arrays are written similarly to lists, but with a leading `#`:
+```Lean
+{{#example_decl Examples/Classes.lean northernTrees}}
+```
+The number of values in an array can be found using `Array.size`.
+For instance, `{{#example_in Examples/Classes.lean northernTreesSize}}` evaluates to `{{#example_out Examples/Classes.lean northernTreesSize}}`.
+For indices that are smaller than an array's size, indexing notation can be used to find the corresponding value, just as with lists.
+That is, `{{#example_in Examples/Classes.lean northernTreesTwo}}` evaluates to `{{#example_out Examples/Classes.lean northernTreesTwo}}`.
+Similarly, the compiler requires a proof that an index is in bounds, and attempting to look up a value outside the bounds of the array results in a compile-time error, just as with lists.
+For instance, `{{#example_in Examples/Classes.lean northernTreesEight}}` results in:
+```Lean error
+{{#example_out Examples/Classes.lean northernTreesEight}}
+```
+
+## Non-Empty Lists
+
+A datatype that represents non-empty lists can be defined as a structure with a field for the head of the list and a field for the tail, which is a potentially empty list:
+```Lean
+{{#example_decl Examples/Classes.lean NonEmptyList}}
+```
+For instance, the non-empty list `idahoSpiders` (which contains some spider species native to the US state of Idaho) consists of `{{#example_out Examples/Classes.lean firstSpider}}` followed by four other spiders, for a total of five spiders.
+
+Looking up the value at a specific index in this list with a recursive function should consider three possibilities:
+ 1. The index is `0`, in which case the head of the list should be returned.
+ 2. The index is `n + 1` and the tail is empty, in which case the index is out of bounds.
+ 3. The index is `n + 1` and the tail is non-empty, in which case the function can be called recursively on the tail and `n`.
+
+For example, a lookup function that returns an `Option` can be written as follows:
+```Lean
+{{#example_decl Examples/Classes.lean NEListGetHuh}}
+```
+The recursive call to `get?` does not require a `NonEmptyList` namespace qualifier because the body of the definition is implicitly in the definition's namespace.
+Another way to write this function uses `get?` for lists when the index is greater than zero:
+```Lean
+{{#example_decl Examples/Classes.lean NEListGetHuhList}}
+```
+
+If the list contains one entry, then only `0` is a valid index.
+If it contains two entries, then both `0` and `1` are valid indices.
+If it contains three entries, then `0`, `1`, and `2` are valid indices.
+In other words, the valid indices into a non-empty list are natural numbers less than or equal to the length of the tail.
+
+The definition of what it means for an index to be in bounds should be written as an `abbrev` because the tactics used to find evidence that indices are acceptable are able to solve inequalities of numbers, but they don't know anything about the name `NonEmptyList.inBounds`:
+```Lean
+{{#example_decl Examples/Classes.lean inBoundsNEList}}
+```
+This function returns a proposition that might be true or false.
+For instance, `2` is in bounds for `idahoSpiders`, while `5` is not:
+```
+{{#example_decl Examples/Classes.lean spiderBoundsChecks}}
+```
+The logical negation operator has a very low precedence, which means that `¬idahoSpiders.inBounds 5` is equivalent to `¬(idahoSpiders.inBounds 5)`.
+
+
+This fact can be used to write a lookup function that requires evidence that the index is valid, and thus need not return `Option`, by delegating to the version for lists that checks the evidence at compile time:
+```Lean
+{{#example_decl Examples/Classes.lean NEListGet}}
+```
+It is, of course, possible to write this function to use the evidence directly, rather than delegating to a standard library function that happens to be able to use the same evidence.
+This requires techniques for working with proofs and propositions that are described later in this book.
+
+
+## Overloading Indexing
+
+Indexing notation for a collection type can be overloaded by defining an instance of the `GetElem` type class.
+For the sake of flexiblity, `GetElem` has four parameters:
+ * The type of the collection
+ * The type of the index
+ * The type of elements that are extracted from the collection
+ * A function that determines the appropriate evidence that the index is in bounds
+The element type and the evidence function are both output parameters.
+`GetElem` has a single method, `getElem`, which takes a collection value, an index value, and evidence that the index is in bounds as arguments, and returns an element.
+ 
+In the case of `NonEmptyList α`, these parameters are:
+ * The collection is `NonEmptyList α`
+ * Indices have type `Nat`
+ * The type of elements is `α`
+ * An index is in bounds if it is less than or equal to the length of the tail
+
+In fact, the `GetElem` instance can delegate directly to `NonEmptyList.get`:
+```Lean
+{{#example_decl Examples/Classes.lean GetElemNEList}}
+```
+With this instance, `NonEmptyList` becomes just as convenient to use as `List`.
+Evaluating `{{#example_in Examples/Classes.lean firstSpider}}` yields `{{#example_out Examples/Classes.lean firstSpider}}`, while `{{#example_in Examples/Classes.lean tenthSpider}}` leads to the compile-time error:
+```Lean error
+{{#example_out Examples/Classes.lean tenthSpider}}
+```
+
+Because both the collection type and the index type are input parameters to the `GetElem` type class, new types can be used to index into existing collections.
+The positive number type `Pos` is a perfectly reasonable index into a `List`, with the caveat that it cannot point at the first entry.
+The follow instance of `GetElem` allows `Pos` to be used just as conveniently as `Nat` to find a list entry:
+```Lean
+{{#example_decl Examples/Classes.lean ListPosElem}}
+```
+
+Indexing can also make sense for non-numeric indices.
+For example, `Bool` can be used to select between the fields in a point, with `false` corresponding to `x` and `true` corresponding to `y`:
+```Lean
+{{#example_decl Examples/Classes.lean PPointBoolGetElem}}
+```
+In this case, both Booleans are valid indices.
+Because every possible `Bool` is in bounds, the evidence is simply the true proposition `True`.
 
